LeanSorting/PartialExamples.lean
@@ -1,0 +1,22 @@
+import «LeanSorting».Partial
+
+-- All of the following should evaluate to 'true'. We can't use 'example' here to test these
+-- more nicely because 'mergeSortPartial' is, well, partial.
+
+#eval #[].mergeSortPartial (α := Nat) = #[]
+#eval #[0].mergeSortPartial = #[0]
+#eval #[0, 1].mergeSortPartial = #[0, 1]
+#eval #[1, 0].mergeSortPartial = #[0, 1]
+#eval #[0, 0].mergeSortPartial = #[0, 0]
+#eval #[1, 1].mergeSortPartial = #[1, 1]
+#eval #[0, 1, 2].mergeSortPartial = #[0, 1, 2]
+#eval #[0, 2, 1].mergeSortPartial = #[0, 1, 2]
+#eval #[1, 0, 2].mergeSortPartial = #[0, 1, 2]
+#eval #[1, 2, 0].mergeSortPartial = #[0, 1, 2]
+#eval #[2, 0, 1].mergeSortPartial = #[0, 1, 2]
+#eval #[2, 1, 0].mergeSortPartial = #[0, 1, 2]
+#eval #[0, 0, 0].mergeSortPartial = #[0, 0, 0]
+#eval #[1, 1, 1].mergeSortPartial = #[1, 1, 1]
+#eval #[2, 2, 2].mergeSortPartial = #[2, 2, 2]
+#eval #[10, 9, 8, 7, 6, 5, 4, 3, 2, 1].mergeSortPartial = #[1, 2, 3, 4, 5, 6, 7, 8, 9, 10]
+#eval #[10, 0, 100, 1, 200, 2].mergeSortPartial = #[0, 1, 2, 10, 100, 200]
