Main.lean
@@ -1,4 +1,6 @@
 import «LeanSorting».Total
+import «LeanSorting».Partial
+import Mathlib.Data.BinaryHeap
 
 def getLines : IO (Array String) := do
   let stdin ← IO.getStdin
@@ -17,8 +19,9 @@ def mainSort (sort : Array String → Array String) : IO Unit := do
 
 def main (args : List String) : IO UInt32 := do
   match args with
-  | ["--msort"] => mainSort Array.mergeSort; pure 0
-  | ["--msort-partial"] => mainSort Array.mergeSortPartial; pure 0
+  | ["--mergeSort"] => mainSort Array.mergeSort; pure 0
+  | ["--mergeSortPartial"] => mainSort Array.mergeSortPartial; pure 0
+  | ["--heapSort"] => mainSort (Array.heapSort · (· < ·)); pure 0
   | ["--qsort"] => mainSort (Array.qsort · (· < ·)); pure 0
   | _ =>
     IO.println "Expected single argument, either \"--msort\" or \"--qsort\""
